# baseURI: http://def.seegrid.csiro.au/ontology/time-plus
# imports: http://www.w3.org/2006/time

@prefix : <http://def.seegrid.csiro.au/ontology/time-plus#> .
@prefix geotime: <http://resource.geosciml.org/classifier/ics/ischart/> .
@prefix my: <http://example.org/my/> .
@prefix owl: <http://www.w3.org/2002/07/owl#> .
@prefix rdf: <http://www.w3.org/1999/02/22-rdf-syntax-ns#> .
@prefix rdfs: <http://www.w3.org/2000/01/rdf-schema#> .
@prefix time: <http://www.w3.org/2006/time#> .
@prefix tzont: <http://www.w3.org/2006/timezone#> .
@prefix xsd: <http://www.w3.org/2001/XMLSchema#> .

<http://def.seegrid.csiro.au/ontology/geotime/EndOfDinosaurs>
  rdf:type time:Instant ;
  :inTimePosition geotime:BaseCenozoic ;
  :inTimePosition [
      rdf:type :TimePosition ;
      :textValue "Base of Cenozoic"^^xsd:string ;
      :trs geotime: ;
    ] ;
  rdfs:label "End of the age of dinosaurs"^^xsd:string ;
.
<http://def.seegrid.csiro.au/ontology/geotime/FormationOfEarth>
  rdf:type time:Instant ;
  :inTimePosition [
      rdf:type :TimePosition ;
      :numericValue 4.567e9 ;
      :trs <http://example.org/trs/ybp> ;
    ] ;
  rdfs:label "Formation of the earth"^^xsd:string ;
.
<http://def.seegrid.csiro.au/ontology/time-plus>
  rdf:type owl:Ontology ;
  owl:imports <http://www.w3.org/2006/time> ;
  owl:versionInfo "Created with TopBraid Composer"^^xsd:string ;
.
:DateTimeDescription
  rdf:type owl:Class ;
  rdfs:comment "Clone of W3C Time time:DateTimeDescription, to allow non-Gregorian day/month/year values. :day :month :year properties are replaced with properties that permit essentially the same lexical pattern, but without the requirement that they denote Gregorian calendar elements."^^xsd:string ;
  rdfs:subClassOf [
      rdf:type owl:Restriction ;
      owl:cardinality "1"^^xsd:nonNegativeInteger ;
      owl:onProperty :trs ;
    ] ;
  rdfs:subClassOf [
      rdf:type owl:Restriction ;
      owl:cardinality "1"^^xsd:nonNegativeInteger ;
      owl:onProperty time:unitType ;
    ] ;
  rdfs:subClassOf [
      rdf:type owl:Restriction ;
      owl:maxCardinality "1"^^xsd:nonNegativeInteger ;
      owl:onProperty :day ;
    ] ;
  rdfs:subClassOf [
      rdf:type owl:Restriction ;
      owl:maxCardinality "1"^^xsd:nonNegativeInteger ;
      owl:onProperty :month ;
    ] ;
  rdfs:subClassOf [
      rdf:type owl:Restriction ;
      owl:maxCardinality "1"^^xsd:nonNegativeInteger ;
      owl:onProperty :year ;
    ] ;
  rdfs:subClassOf [
      rdf:type owl:Restriction ;
      owl:maxCardinality "1"^^xsd:nonNegativeInteger ;
      owl:onProperty time:dayOfWeek ;
    ] ;
  rdfs:subClassOf [
      rdf:type owl:Restriction ;
      owl:maxCardinality "1"^^xsd:nonNegativeInteger ;
      owl:onProperty time:dayOfYear ;
    ] ;
  rdfs:subClassOf [
      rdf:type owl:Restriction ;
      owl:maxCardinality "1"^^xsd:nonNegativeInteger ;
      owl:onProperty time:hour ;
    ] ;
  rdfs:subClassOf [
      rdf:type owl:Restriction ;
      owl:maxCardinality "1"^^xsd:nonNegativeInteger ;
      owl:onProperty time:minute ;
    ] ;
  rdfs:subClassOf [
      rdf:type owl:Restriction ;
      owl:maxCardinality "1"^^xsd:nonNegativeInteger ;
      owl:onProperty time:second ;
    ] ;
  rdfs:subClassOf [
      rdf:type owl:Restriction ;
      owl:maxCardinality "1"^^xsd:nonNegativeInteger ;
      owl:onProperty time:timeZone ;
    ] ;
  rdfs:subClassOf [
      rdf:type owl:Restriction ;
      owl:maxCardinality "1"^^xsd:nonNegativeInteger ;
      owl:onProperty time:week ;
    ] ;
.
:TRS
  rdf:type owl:Class ;
  rdfs:comment "Temporal Reference System"^^xsd:string ;
  rdfs:label "Temporal Reference System"^^xsd:string ;
.
:TimePosition
  rdf:type owl:Class ;
  rdfs:comment "Alternative to time:DateTimeDescription and xsd:dateTime to support description of a temporal position outside the Julian calendar"^^xsd:string ;
  rdfs:comment "Position within a specified Temporal Reference System"^^xsd:string ;
  rdfs:label "Temporal position"^^xsd:string ;
  rdfs:subClassOf [
      rdf:type owl:Class ;
      owl:unionOf (
          [
            rdf:type owl:Restriction ;
            owl:cardinality "1"^^xsd:nonNegativeInteger ;
            owl:onProperty :numericValue ;
          ]
          [
            rdf:type owl:Restriction ;
            owl:cardinality "1"^^xsd:nonNegativeInteger ;
            owl:onProperty :textValue ;
          ]
        ) ;
    ] ;
  rdfs:subClassOf [
      rdf:type owl:Restriction ;
      owl:cardinality "1"^^xsd:nonNegativeInteger ;
      owl:onProperty :trs ;
    ] ;
.
:day
  rdf:type owl:DatatypeProperty ;
  rdfs:comment "Clone of W3C Time time:day, modified to support non-Gregorian day values. The range of this property is a string pattern with essentially the same lexical form as time:day, but without the requirement that it denotes a Gregorian calendar day. "^^xsd:string ;
  rdfs:domain :DateTimeDescription ;
  rdfs:range [
      rdf:type rdfs:Datatype ;
      owl:onDataType xsd:string ;
      owl:withRestrictions (
          [
            xsd:pattern "---[0-9]+"^^xsd:string ;
          ]
        ) ;
    ] ;
.
:inDateTime
  rdf:type owl:ObjectProperty ;
  rdfs:comment "Clone of W3C Time time:inDateTime, modified to support non-Gregorian values."^^xsd:string ;
  rdfs:domain time:Instant ;
  rdfs:range :DateTimeDescription ;
.
:inTimePosition
  rdf:type owl:ObjectProperty ;
  rdfs:comment "Position of a time instant expressed as a TimePosition"^^xsd:string ;
  rdfs:domain time:Instant ;
  rdfs:label "Temporal position"^^xsd:string ;
  rdfs:range :TimePosition ;
.
:month
  rdf:type owl:DatatypeProperty ;
  rdfs:comment "Clone of W3C Time time:month, modified to support non-Gregorian month values. The range of this property is a string pattern with essentially the same lexical form as time:month, but without the requirement that it denotes a Gregorian calendar month."^^xsd:string ;
  rdfs:domain :DateTimeDescription ;
  rdfs:range [
      rdf:type rdfs:Datatype ;
      owl:onDataType xsd:string ;
      owl:withRestrictions (
          [
            xsd:pattern "--[0-9]+"^^xsd:string ;
          ]
        ) ;
    ] ;
.
:numericValue
  rdf:type owl:DatatypeProperty ;
  rdfs:comment "Value of a TimePosition within a specified reference frame expressed as a number"^^xsd:string ;
  rdfs:domain :TimePosition ;
  rdfs:label "Numeric value of temporal position"^^xsd:string ;
  rdfs:range [
      rdf:type rdfs:DataType ;
      owl:unionOf (
          xsd:decimal
          xsd:float
          xsd:double
        ) ;
    ] ;
.
:textValue
  rdf:type owl:DatatypeProperty ;
  rdfs:comment "Value of a TimePosition within a specified reference frame expressed as a text value or label"^^xsd:string ;
  rdfs:domain :TimePosition ;
  rdfs:label "Text value of temporal position"^^xsd:string ;
  rdfs:range xsd:string ;
.
:trs
  rdf:type owl:ObjectProperty ;
  rdfs:comment "Reference system used for the temporal position"^^xsd:string ;
  rdfs:domain [
      rdf:type owl:Class ;
      owl:unionOf (
          time:DateTimeDescription
          :DateTimeDescription
          :TimePosition
        ) ;
    ] ;
  rdfs:label "Temporal reference system used"^^xsd:string ;
  rdfs:range :TRS ;
.
:year
  rdf:type owl:DatatypeProperty ;
  rdfs:comment "Clone of W3C Time time:year, modified to support non-Gregorian year values. The range of this property is a string pattern with essentially the same lexical form as time:year, but without the requirement that it denotes a Gregorian calendar year."^^xsd:string ;
  rdfs:domain :DateTimeDescription ;
  rdfs:range xsd:integer ;
.
my:AbbyBirthday
  rdf:type time:Instant ;
  :inDateTime my:AbbyBirthdayHebrew ;
  :inTimePosition my:AbbyBirthdayUnix ;
  rdfs:label "Abby's birthdate"^^xsd:string ;
  time:inDateTime my:AbbyBirthdayGregorian ;
  time:inXSDDateTime "2001-05-23T08:20:00+08:00"^^xsd:dateTime ;
.
my:AbbyBirthdayGregorian
  rdf:type time:DateTimeDescription ;
  time:day "---23"^^xsd:gDay ;
  time:dayOfWeek time:Wednesday ;
  time:hour "8"^^xsd:nonNegativeInteger ;
  time:minute "20"^^xsd:nonNegativeInteger ;
  time:month "--05"^^xsd:gMonth ;
  time:timeZone [
      rdf:type tzont:TimeZone ;
      tzont:GMToffset "+8" ;
      tzont:name "AWST" ;
    ] ;
  time:unitType time:unitMinute ;
  time:year "2001"^^xsd:gYear ;
.
my:AbbyBirthdayHebrew
  rdf:type :DateTimeDescription ;
  :day "---01" ;
  :month "--03" ;
  :trs <http://dbpedia.org/resource/Hebrew_calendar> ;
  :year 5761 ;
  time:unitType time:unitDay ;
.
my:AbbyBirthdayUnix
  rdf:type :TimePosition ;
  :numericValue 990577200 ;
  :trs <http://dbpedia.org/resource/Unix_time> ;
  rdfs:label "Abby's birthdate in Unix time"^^xsd:string ;
.
geotime:BaseOrdovician
  rdf:type time:Instant ;
  :inTimePosition geotime:BaseOrdovicianTime ;
  rdfs:label "Base of Ordovician Period"^^xsd:string ;
.
geotime:BaseOrdovicianTime
  rdf:type :TimePosition ;
  :numericValue 485.4 ;
  :trs <http://resource.geosciml.org/classifier/cgi/geologicage/ma> ;
  rdfs:label "Position of Base of Ordovician Period"^^xsd:string ;
.
geotime:BasePhanerozoic
  rdf:type time:Instant ;
  :inTimePosition geotime:BasePhanerozoicTime ;
  rdfs:label "Base of Phanerozoic Eon"^^xsd:string ;
.
geotime:BasePhanerozoicTime
  rdf:type :TimePosition ;
  :numericValue 541.0 ;
  :trs <http://resource.geosciml.org/classifier/cgi/geologicage/ma> ;
  rdfs:label "Position of Base of Phanerozoic Eon"^^xsd:string ;
.
geotime:Cambrian
  rdf:type time:ProperInterval ;
  rdfs:label "Cambrian period"^^xsd:string ;
  time:hasBeginning geotime:BasePhanerozoic ;
  time:hasEnd geotime:BaseOrdovician ;
  time:intervalAfter geotime:Precambrian ;
  time:intervalBefore geotime:Mesozoic ;
  time:intervalBefore geotime:Ordovician ;
  time:intervalBefore geotime:Silurian ;
  time:intervalContains geotime:CambrianSeries2 ;
  time:intervalContains geotime:CambrianSeries3 ;
  time:intervalFinishedBy geotime:Furongian ;
  time:intervalMeets geotime:Ordovician ;
  time:intervalMeets geotime:Precambrian ;
  time:intervalStartedBy geotime:Terreneuvian ;
  time:intervalStarts geotime:Paleozoic ;
  time:intervalStarts geotime:Phanerozoic ;
.
